Fixed Congruence Bugs

trunk/source/AbstractInterpretationV2/src/de/uni_freiburg/informatik/ultimate/plugins/analysis/abstractinterpretationv2/domain/nonrelational/congruence/CongruenceDomainStatementProcessor.java
@@ -108,17 +108,8 @@ public class CongruenceDomainStatementProcessor extends BoogieVisitor {
 		mOldState = oldState;
 
 		mLhsVariable = null;
-
-		// Use the overridden version of the BoogieVisitor (calls ExpressionTransformer just once)
-		Statement transformedStatement = new TransformedVisitor().processStatement(statement);
 		
-		if (transformedStatement != statement && mLogger.isDebugEnabled()) {
-			mLogger.debug(new StringBuilder().append(AbsIntPrefInitializer.INDENT).append(" Statement ")
-			        .append(BoogiePrettyPrinter.print(statement)).append(" rewritten to: ")
-			        .append(BoogiePrettyPrinter.print(transformedStatement)));
-		}
-		
-		processStatement(transformedStatement);
+		processStatement(statement);
 
 		assert mReturnState.size() != 0;
 
@@ -150,7 +141,14 @@ public class CongruenceDomainStatementProcessor extends BoogieVisitor {
 			mExpressionEvaluator.addEvaluator(new CongruenceSingletonValueExpressionEvaluator(new CongruenceDomainValue()));
 			return expr;
 		}
-		return super.processExpression(expr);
+		final ExpressionTransformer t = new ExpressionTransformer();
+		Expression newExpr = t.transform(expr);
+		if (!newExpr.toString().equals(expr.toString()) && mLogger.isDebugEnabled()) {
+			mLogger.debug(new StringBuilder().append(AbsIntPrefInitializer.INDENT).append(" Expression ")
+			        .append(BoogiePrettyPrinter.print(expr)).append(" rewritten to: ")
+			        .append(BoogiePrettyPrinter.print(newExpr)));
+		}
+		return super.processExpression(newExpr);
 	}
 
 	private void handleAssignment(final AssignmentStatement statement) {
@@ -413,19 +411,5 @@ public class CongruenceDomainStatementProcessor extends BoogieVisitor {
 
 		// This expression should be added first to the evaluator inside the handling of processExpression.
 		processExpression(newUnary);
-	}
-
-	private final static class TransformedVisitor extends BoogieVisitor{
-		@Override
-		protected Statement processStatement(Statement statement) {
-			return super.processStatement(statement);
-		}
-		
-		@Override
-		protected Expression processExpression(Expression expr) {
-			final ExpressionTransformer t = new ExpressionTransformer();
-			return t.transform(expr);
-		}
-	}
-	
+	}	
 }
